
Let $\mathcal{R} = \mathsf{UniverseR} (X)$. In the following, the set
comprehension represents the requirements of valuations. For instance,
the notation $\{ R_{[v]} | D_1 \neq D_1 \}$ denotes the set 
$\{ R_{[v]} | v (D_1) \neq v (D_2) \}$. The following table shows the
details of computation.

{\begin{tabular}{|c|l|}
  \hline
  $U_0$ & $L \times \{ R_{[v]} | D_1 \neq D_2\}$ \\
  \hline
  $W_0$ & 
  $
  \begin{array}{lr}
    \{ l_0, l_1, L_1, L_{3} \} \times \mathcal{R} & \cup\\
    \left\{
      \begin{array}{l|l}
        \multirow{2}{*}{ $\langle l_2, R_{[v]} \rangle $ } &
        (r_2 = s \wedge D_1\neq s) \vee 
        (r_2 = t \wedge D_1 \neq t) \vee 
        (s = t \wedge D_1 \neq s) \vee \\
        & (r_2 \neq s \wedge r_2 \neq t \wedge s \neq t \wedge D_1 \neq 0)
      \end{array}
    \right\} & \cup\\
    \{ \langle L_2, R_{[v]} \rangle | D_1 \neq D_2 \}
  \end{array}
  $\\
  \hline
  $U_1$ & 
  $
  \begin{array}{lr}
    \{ l_0, l_1, L_1, L_{3} \} \times \{R_{[v]} | D_1 \neq D_2\} & \cup \\
    \left\{
      \begin{array}{l|l}
        \multirow{3}{*}{ $ \langle l_2, R_{[v]} \rangle $ } &
        (D_1 \neq D_2) \wedge \\
        &
        ((r_2 = s \wedge D_1 \neq s) \vee (r_2 = t \wedge D_1\neq t) \vee
         (s = t \wedge D_1 \neq s) \vee\\
         &
         (r_2 \neq s \wedge r_2 \neq t \wedge s \neq t \wedge D_1 \neq 0))
      \end{array}
    \right\} & \cup\\
    \{ \langle L_2, R_{[v]} \rangle | D_1 \neq D_2\}
  \end{array}
  $\\
  \hline
  $W_1$ &
  $
  \begin{array}{lr}
    \{ l_0, l_1, L_1 \} \times \mathcal{R} & \cup \\
    \{ \langle L_3, R_{[v]} \rangle |
    (D_1 \neq r_2) \vee (D_1 \neq 0 \wedge r_1\neq r_2) \} & \cup\\
    \left\{
      \begin{array}{l|l}
        \multirow{3}{*}{ $ \langle l_2, R_{[v]} \rangle $ } &
        (D_1 \neq D_2) \wedge \\
        &
        ((r_2 = s \wedge D_1 \neq s) \vee (r_2 = t \wedge D_1\neq t) \vee
         (s = t \wedge D_1 \neq s) \vee\\
         &
         (r_2 \neq s \wedge r_2 \neq t \wedge s \neq t \wedge D_1 \neq 0))
      \end{array}
    \right\} & \cup\\
    \{ \langle L_2, R_{[v]} \rangle | D_1 \neq D_2\}
  \end{array}
  $
  \\
  \hline
  $U_2$ &
  $
  \begin{array}{lr}
    \{ l_0, l_1, L_1 \} \times \{R_{[v]} | D_1 \neq D_2\} & \cup \\
    \{ \langle L_3, R_{[v]} \rangle |
    (D_1 \neq D_2) \wedge (D_1 \neq r_2) \vee
    (D_1 \neq 0 \wedge r_1 \neq r_2))\} & \cup\\
    \left\{
      \begin{array}{l|l}
        \multirow{3}{*}{ $ \langle l_2, R_{[v]} \rangle $ } &
        (D_1 \neq D_2) \wedge \\
        &
        ((r_2 = s \wedge D_1 \neq s) \vee (r_2 = t \wedge D_1\neq t) \vee
         (s = t \wedge D_1 \neq s) \vee\\
         &
         (r_2 \neq s \wedge r_2 \neq t \wedge s \neq t \wedge D_1 \neq 0))
      \end{array}
    \right\} & \cup\\
    \{ \langle L_2, R_{[v]} \rangle | D_1 \neq D_2\}
  \end{array}
  $
  \\
  \hline
  $W_2$ &
  $
  \begin{array}{lr}
    \{ l_0, l_1 \} \times \mathcal{R} & \cup\\
    \{ \langle L_1, R_{[v]} \rangle |
    (D_1 \neq r_2) \vee (D_1 \neq 0 \wedge r_1 \neq r_2) \} & \cup\\
    \{ \langle L_3, R_{[v]} \rangle |
    (D_1 \neq D_2) \wedge (D_1 \neq r_2) \vee
    (D_1 \neq 0 \wedge r_1 \neq r_2))\} & \cup\\
    \left\{
      \begin{array}{l|l}
        \multirow{3}{*}{ $ \langle l_2, R_{[v]} \rangle $ } &
        (D_1 \neq D_2) \wedge \\
        &
        ((r_2 = s \wedge D_1 \neq s) \vee (r_2 = t \wedge D_1\neq t) \vee
         (s = t \wedge D_1 \neq s) \vee\\
         &
         (r_2 \neq s \wedge r_2 \neq t \wedge s \neq t \wedge D_1 \neq 0))
      \end{array}
    \right\} & \cup\\
    \{ \langle L_2, R_{[v]} \rangle | D_1 \neq D_2\}
  \end{array}
  $
  \\
  \hline
  $U_3$ &
  $
  \begin{array}{lr}
    \{ l_0, l_1 \} \times \{ R_{[v]} | D_1 \neq D_2\} & \cup \\
    \{ \langle L_1, R_{[v]} \rangle |
    (D_1 \neq D_2) \wedge 
    ((D_1 \neq r_2) \vee (D_1 \neq r_1) \vee 
    (D_1 \neq 0 \wedge r_1 \neq r_2))\} & \cup\\
    \{ \langle L_3, R_{[v]} \rangle |
    (D_1 \neq D_2) \wedge (D_1 \neq r_2) \vee
    (D_1 \neq 0 \wedge r_1 \neq r_2))\} & \cup\\
    \left\{
      \begin{array}{l|l}
        \multirow{3}{*}{ $ \langle l_2, R_{[v]} \rangle $ } &
        (D_1 \neq D_2) \wedge \\
        &
        ((r_2 = s \wedge D_1 \neq s) \vee (r_2 = t \wedge D_1\neq t) \vee
         (s = t \wedge D_1 \neq s) \vee\\
         &
         (r_2 \neq s \wedge r_2 \neq t \wedge s \neq t \wedge D_1 \neq 0))
      \end{array}
    \right\} & \cup\\
    \{ \langle L_2, R_{[v]} \rangle | D_1 \neq D_2\}
  \end{array}
  $
  \\
  \hline
      \end{tabular}
}

{\small
\begin{tabular}{|c|l|}
\hline
  $W_3$ &
  $
  \begin{array}{lr}
    \{ l_0 \} \times \mathcal{R} & \cup \\
    \left\{ 
      \begin{array}{l|l}
        \multirow{4}{*}{ $\langle l_1, R_{[v]} \rangle$ }
        & 
        [(r_1 = s \wedge s \neq r_2) \vee (r_1 = t \wedge t \neq r_2) \vee
         (s = t \wedge s \neq r_2) \vee \\
        & \ \ \ \ 
        (r_1 \neq s \wedge r_1 \neq t \wedge s \neq t \wedge r_2 \neq 0)] 
        \vee\\
        & 
        [(r_1 = s \wedge s \neq 0 \wedge r_1 \neq r_2) \vee
         (r_1 =t \wedge t \neq 0 \wedge r_1 \neq r_2) \vee\\
        & \ \ \ \ 
         (s = t \wedge s \neq 0 \wedge r_1 \neq r_2)]
      \end{array}
    \right\}    & \cup\\
    \{ \langle L_1, R_{[v]} \rangle |
    (D_1 \neq D_2) \wedge 
    ((D_1 \neq r_2) \vee (D_1 \neq r_1) \vee 
    (D_1 \neq 0 \wedge r_1 \neq r_2))\} & \cup\\
    \{ \langle L_3, R_{[v]} \rangle |
    (D_1 \neq D_2) \wedge (D_1 \neq r_2) \vee
    (D_1 \neq 0 \wedge r_1 \neq r_2))\} & \cup\\
    \left\{
      \begin{array}{l|l}
        \multirow{3}{*}{ $ \langle l_2, R_{[v]} \rangle $ } &
        (D_1 \neq D_2) \wedge \\
        &
        ((r_2 = s \wedge D_1 \neq s) \vee (r_2 = t \wedge D_1\neq t) \vee
         (s = t \wedge D_1 \neq s) \vee\\
         &
         (r_2 \neq s \wedge r_2 \neq t \wedge s \neq t \wedge D_1 \neq 0))
      \end{array}
    \right\} & \cup\\
    \{ \langle L_2, R_{[v]} \rangle | D_1 \neq D_2\}
  \end{array}
  $
  \\
  \hline
  $U_4$ &
  $
  \begin{array}{lr}
    \{ \langle l_0, R_{[v]} \rangle | D_1 \neq D_2\} & \cup \\
    \left\{
      \begin{array}{l|l}
        \multirow{5}{*}{ $\langle l_1, R_{[v]} \rangle$ } &
        (D_1 \neq D_2) \wedge \\
        &
        ([(r_1 = s \wedge s \neq r_2) \vee 
          (r_1 = t \wedge t \neq r_2) \vee
          (s = t \wedge s \neq r_2) \vee \\
        & \ \ \ \ 
          (r_1 \neq s \wedge r_1 \neq t \wedge s \neq t \wedge r_2 \neq 0)]
        \vee\\
        &
         \ [(r_1 = s \wedge s \neq 0 \wedge r_1 \neq r_2) \vee
          (r_1 = t \wedge t \neq 0 \wedge r_1 \neq r_2) \vee \\
        & \ \ \ \ 
          (s = t \wedge s \neq 0 \wedge r_1 \neq r_2)])\\
      \end{array}
      \right\} & \cup\\
    \{ \langle L_1, R_{[v]} \rangle |
    (D_1 \neq D_2) \wedge 
    ((D_1 \neq r_2) \vee (D_1 \neq r_1) \vee 
    (D_1 \neq 0 \wedge r_1 \neq r_2))\} & \cup\\
    \{ \langle L_3, R_{[v]} \rangle |
    (D_1 \neq D_2) \wedge (D_1 \neq r_2) \vee
    (D_1 \neq 0 \wedge r_1 \neq r_2))\} & \cup\\
    \left\{
      \begin{array}{l|l}
        \multirow{3}{*}{ $ \langle l_2, R_{[v]} \rangle $ } &
        (D_1 \neq D_2) \wedge \\
        &
        ((r_2 = s \wedge D_1 \neq s) \vee (r_2 = t \wedge D_1\neq t) \vee
         (s = t \wedge D_1 \neq s) \vee\\
         &
         (r_2 \neq s \wedge r_2 \neq t \wedge s \neq t \wedge D_1 \neq 0))
      \end{array}
    \right\} & \cup\\
    \{ \langle L_2, R_{[v]} \rangle | D_1 \neq D_2\}
  \end{array}
  $
  \\
  \hline

  $W_4$ &
  $
  \begin{array}{lr}
    \{ \langle l_0, R_{[v]} \rangle | r_1 \neq r_2\} & \cup\\
    \left\{
      \begin{array}{l|l}
        \multirow{5}{*}{ $\langle l_1, R_{[v]} \rangle$ } &
        (D_1 \neq D_2) \wedge \\
        &
        ([(r_1 = s \wedge s \neq r_2) \vee 
          (r_1 = t \wedge t \neq r_2) \vee
          (s = t \wedge s \neq r_2) \vee \\
        & \ \ \ \ 
          (r_1 \neq s \wedge r_1 \neq t \wedge s \neq t \wedge r_2 \neq 0)]
        \vee\\
        &
         \ [(r_1 = s \wedge s \neq 0 \wedge r_1 \neq r_2) \vee
          (r_1 = t \wedge t \neq 0 \wedge r_1 \neq r_2) \vee \\
        & \ \ \ \ 
          (s = t \wedge s \neq 0 \wedge r_1 \neq r_2)])\\
      \end{array}
      \right\} & \cup\\
    \{ \langle L_1, R_{[v]} \rangle |
    (D_1 \neq D_2) \wedge 
    ((D_1 \neq r_2) \vee (D_1 \neq r_1) \vee 
    (D_1 \neq 0 \wedge r_1 \neq r_2))\} & \cup\\
    \{ \langle L_3, R_{[v]} \rangle |
    (D_1 \neq D_2) \wedge (D_1 \neq r_2) \vee
    (D_1 \neq 0 \wedge r_1 \neq r_2))\} & \cup\\
    \left\{
      \begin{array}{l|l}
        \multirow{3}{*}{ $ \langle l_2, R_{[v]} \rangle $ } &
        (D_1 \neq D_2) \wedge \\
        &
        ((r_2 = s \wedge D_1 \neq s) \vee (r_2 = t \wedge D_1\neq t) \vee
         (s = t \wedge D_1 \neq s) \vee\\
         &
         (r_2 \neq s \wedge r_2 \neq t \wedge s \neq t \wedge D_1 \neq 0))
      \end{array}
    \right\} & \cup\\
    \{ \langle L_2, R_{[v]} \rangle | D_1 \neq D_2\} 
  \end{array}
  $
  \\
  \hline
\end{tabular}
}

Finally, the following representative configurations satisfy $EG \neg
(D_1 = D_2)$.
\begin{equation*}
  \begin{array}{ll}
    \{ \langle l_0, R_{[v]} \rangle | D_1 \neq D_2 \wedge r_1 \neq r_2 \} & 
    \cup \\
    \left\{
      \begin{array}{l|l}
        \multirow{5}{*}{$ \langle l_1, R_{[v]} \rangle$} & 
        (D_1 \neq D_2) \wedge\\
        &
        ([(r_1 = s \wedge s \neq r_2) \vee 
          (r_1 = t \wedge t \neq r_2) \vee
          (s = t \wedge s \neq r_2) \vee\\
        & \ \ \ \ 
          (r_1 \neq s \wedge r_1 \neq t \wedge s \neq t \wedge r_2 \neq 0)]
          \vee\\
        &
        \ [(r_1 = s \wedge s \neq 0 \wedge r_1 \neq r_2) \vee
           (r_1 = t \wedge t \neq 0 \wedge r_1 \neq r_2) \vee \\
        &  \ \ \ 
           (s = t \wedge s \neq 0 \wedge r_1 \neq r_2)])
      \end{array}
    \right\} & 
    \cup \\
    \{ \langle L_1, R_{[v]} \rangle | (D_1 \neq D_2) \wedge 
                ((D_1 \neq r_2) \vee (D_1 \neq 0 \wedge r_1 \neq r_2))\} & 
    \cup\\
    \{ \langle L_3, R_{[v]} \rangle | (D_1 \neq D_2) \wedge 
                ((D_1\neq r_2) \vee (D_1 \neq 0 \wedge r_1 \neq r_2))\} &
    \cup\\
    \left\{
    \begin{array}{l|l}
      \multirow{3}{*}{ $ \langle l_2, R_{[v]} \rangle $ } & 
      (D_1 \neq D_2) \wedge\\
      &
      [(r_2 = s \wedge D_1 \neq s) \vee
       (r_2 = t \wedge D_1 \neq t) \vee
       (s = t \wedge D_1 \neq s) \vee\\
      & \ \ \ \ 
       (r_2 \neq s \wedge r_2 \neq t \wedge s \neq t \wedge D_1\neq 0)]
    \end{array}
    \right\} &
    \cup \\
    \{ \langle L_2, R_{[v]} \rangle | D_1 \neq D_2\}
  \end{array}
\end{equation*}

