

\documentclass[10pt]{IEEEtran}
\usepackage{amsfonts,amsmath}
\usepackage{amssymb, amsmath, graphicx, epsfig, cite,subfigure,color,float}


\vfuzz2pt 

\newtheorem{theorem}{Theorem}[section]
 \newtheorem{corollary}[theorem]{Corollary}
 \newtheorem{lemma}[theorem]{Lemma}
 \newtheorem{proposition}[theorem]{Proposition}
\newtheorem{example}[theorem]{Example}
 \newtheorem{definition}[theorem]{Definition}
 \newtheorem{remark}[theorem]{Remark}
 
\newcommand{\BlackBox}{\rule{1.5ex}{1.5ex}}  \newenvironment{proof}{\par\noindent{\bf Proof\
}}{\hfill\BlackBox\\label{lossless-battery}
  \rm
{\mathcal L}_i(\rm t)=\{\rm L_i(\rm t) |&  {\rm L}_i(\rm t) = \dot {\rm x}_i(\rm t), {\rm x}_i(t_i) = {\rm S}_i,\nonumber\\ & 0 \leq {\rm x}_i(t)\leq {\rm E}_i, t\geq t_i \}.
\nonumber
{\mathcal L}_i(t)&=&\{L_i(t) |  L_i(t) = \partial x_i(t), x_i(t_i) = S_i, \\
				& &x_i(t) \in \{0,1,\ldots, E_i\}, t\geq t_i \}\label{lossless-battery-discrete}.
(t_i, S_i, E_i)a_i(t)=u(t-t_i),\label{arrivaldef}\label{pop}
L(t)=\sum_{i\in {\cal P}_E}L_i(t)=\sum_{i\in {\cal P}_E}\partial x_i(t) a_i(t).
\label{numberineachstate}
 n_x(t)=\sum_{i\in {\cal P}_E}\delta(x_i(t)-x)a_i(t),~x=1,\ldots,E
\label{apx}
 a_x(t)=\sum_{i\in {\cal P}_E}\delta(S_i-x)  a_i(t).
\label{occur}
L(t) & = \sum_{x=0}^{E}\left[\left(\sum_{x'=x}^{E} \partial n_{x'}(t) \right) - (x+1)\partial a_{x}(t)\right].
\label{nxt2}
n_{x}(t+1)&=  a_x(t+1) + \sum_{x' = 0}^E [d_{x',x}(t)- d_{x,x'}(t)]
\\\label{occur3}
L(t) &= \sum_{x=0}^E \sum_{x'=0}^E (x'-x)\partial d_{x,x'}(t)
\label{nxt}
\partial n_{x}(t)&=\partial a_x(t) + \sum_{x' = 0}^E \partial [d_{x',x}(t)-d_{x,x'}(t)]
\nonumber
{\mathcal L}_E(t) = \left\{L(t) |  L(t) = \sum_{x=0}^E \sum_{x'=0}^E (x'-x)\partial d_{x,x'}(t), \right. &&\\ \left.\partial d_{x,x'}(t) \in \mathbb{Z}^+, \sum_{x' = 1}^{E}\partial d_{x,x'}(t) \leq n_x(t)\right\},&&\label{occur4}

\boldsymbol{\theta}_i \xrightarrow[\mathcal{Q}]{\mbox{Quantize}} \boldsymbol{\theta}_q \xrightarrow[\mathcal{I}] {\mbox{Cluster index}} q.
 \label{occur5} \nonumber
{\mathcal L}(t) = \left\{L(t) |  L(t) = \sum_{q=1}^Q\sum_{x=0}^{E^q} \sum_{x'=0}^{E^q} (x'-x)\partial d^q_{x,x'}(t)\right.\nonumber 
& & \\ \left. \partial d_{x,x'}^q(t) \in \mathbb{Z}^+, \sum_{x' = 1}^{E^q}\partial d_{x,x'}^q(t)\leq n^q_x(t) \right\}& &  \nonumber

n_{x}^q(t)&=  a^q_x(t) + \sum_{x' = 0}^{E^q} [d^q_{x',x}(t-1)- d^q_{x,x'}(t-1)]
\label{totplas}
{\mathcal L}(t)=\left\{L(t)|  L(t) = L^{I}(t) + \sum_{v=1}^V L^v(t), L^v(t) \in {\mathcal L}^v(t) \right\}
\nonumber
{\mathcal L}_i(t_i)&=&\{L_i(t) |  L_i(t) = \partial x_i(t), x_i(t_i) = S_i, \\
				& &x_i(t) \in \{0,1,\ldots, E_i\}, x_i(\chi_i) \geq \rho_i E_i, \nonumber \\
& & -G_i \leq \partial x_i(t) \leq G_i, t\geq t_i \}  \label{lossless-battery-discrete2}

{\mathcal S}_x =\{x - G^q, x - G^q+1, \ldots, x + G^q\};
 \label{occur5} 
{\mathcal L}^v(t) = \Big\{L(t) |  L(t) = \sum_{q=1}^{Q^v}\sum_{x=0}^{E^q} \sum_{x'\in \mathcal S_x}(x'-x)\partial d^q_{x,x'}(t),  & & \nonumber\\ \partial d_{x,x'}^q(t) \in \mathbb{Z}^+,\!\!\sum_{x'\in \mathcal S_x}\partial d_{x,x'}^q(t)\leq n^q_x(t),\nonumber & & \\  n_x^q(\chi^q) = 0, \forall x < \rho^q E^q\Big\},~~~~~~~~~~~~~~~& & 
\label{nx}
n_{x}^q(t)&=  a^q_x(t) + \sum_{x'\in \mathcal S_x}[d^q_{x',x}(t-1)- d^q_{x,x'}(t-1)].
 {\mathcal L}^v(t) \!=\! &\Big\{L(t) |  L(t) \!= \!\sum_{q=1}^{Q^v}\sum_{x=0}^{E^q} \!(x'\!-\!x)\partial d^q_{x,x'}(t)|_{x'=\min\{x+G^q,E^q\}}, \nonumber  \\ 
&\partial d_{x,x'}^q(t) \in \mathbb{Z}^+, \partial d_{x,\min\{x+G^q,E^q\}}^q(t)\leq n^q_x(t),\nonumber \\ 
&  n_x^q(\chi^q) = 0, \forall x < \rho^q E^q\Big\} \label{occur6} 

a_i(t) = u(t- t^{s}_i),~~r_i(t) = u(t- t^{e}_i).

{\mathcal L}_i(t)=\Big\{ L_i(t)&|\partial x_i(t)=-k_i x_i(t) +\alpha_i(t)+ b_i(t) G_i,\label{tcls}\\
					& b_i(t)\in \{0,1\}, L_i(t)=b_i(t)G_i, \forall t \in [t_i^s,t_i^e) \nonumber\\
					&|x_i(t)-x^*_i|\leq B_i/2,~  \forall [t]_{24H} \in [\chi_i^s,\chi_i^e)  \Big\}\nonumber
\alpha_i(t)&=x' - (1- k_i) x  - b_i(t) G_i
P_i(x'|x;t;b_i(t))&=p_{\alpha_i}\left(x'-x(1-k_i)-b_i(t) G_i\right).

{\mathbb E}\{D_{x,x'}^q(t)|n^q_x(t)\}&=\sum_{b=0}^1n_{x,b}^q(t)P^q(x'|x;t;b)

n_{x,0}^q(t) + n_{x,1}^q(t) = n_{x}^q(t).

n^q_x(t)&\!=\!a_x^q(t)\!-\! r_x^q(t)+\!\!\!\!\sum_{x'\in {\mathcal S}^q} \!\!\!D_{x',x}^q(t-1)\!-\!D_{x,x'}^q(t-1).\label{nqxdyn}

\forall |x-x^{*q}|>B^q/2~~\rightarrow~~{\rm Pr}(n_x(t)=0)\geq \eta, 
 \label{occur5} 
{\mathcal L}^v(t) = \Big\{L(t) |  L(t) = \sum_{q=1}^{Q^v} G^q \sum_{x\in {\mathcal S}^q}n_{x,1}^q(t), n_{x,1}^q(t) \in \mathbb{Z}^+&&
\\~n_{x,0}^q(t) + n_{x,1}^q(t) = n_{x}^q(t)~, 
n^q_x(t)=\mbox{see \eqref{nqxdyn}}&&\nonumber\\
{\mathbb E}\{D_{x,x'}^q(t)|n^q_x(t)\}=\sum_{b=0}^1n_{x,b}^q(t)P^q(x'|x;t;b); &&\nonumber\\
\forall x: |x-x^{*q}|>B^q/2,~~\forall [t]_{24H}\in [\chi^{s,q},\chi^{e,q})&&\nonumber\\~~~~~~~~~~~~~~~~~~~~~~~~~\rightarrow~{\rm Pr}(n^q_x(t)=0)\geq \eta \Big\}  \nonumber&&
x_i^*-(-1)^{b_i(t)}\frac{B_i}{2}.
\tau_{i}(t)=\frac 1 {k_i}\ln\left(
\frac{x_i(t)-b_i(t)\frac{G_i}{k_i}-\frac{\alpha_i(t)}{k_i}}
{x_i^*-(-1)^{b_i(t)}\frac{B_i}{2}-b_i(t)\frac{G_i}{k_i}-\frac{\alpha_i(t)}{k_i}}
\right).
\label{coarsecluster}
n_{\tau,b}(t)=\sum_{i\in {\mathcal P}} \delta(\tau-Q(\tau_i(t)))\delta(b-b_i(t))(a_i(t) - r_i(t)).

{\mathcal L}_i(t)=\{L_i(t)| L_i(t)=\ell_i(t-\tau_i),t_i \leq \tau_i \leq t + \chi_i\}

{\mathcal L}_i(t)=&\{L_i(t)| L_i(t)=\ell_i(t)\star \partial x_i(t), x_i(t) \in \{0,1\},\label{eq.defer}\\
	& ~x_i(t)\geq a_i(t-\chi_i), ~x_i(t-1)\leq x_i(t)\leq a_i(t) \}.\nonumber
\label{lint}
{\mathcal L}^v(t) \!=\! \Big\{&L(t) |  L(t) \!= \!\sum_{q=1}^{Q^v} \ell^q(t)\star \partial d^q(t), d^q(t)\in\mathbb{Z}^+ \\ 
& ~d^q(t)\geq a^q(t-\chi^q), ~d^q(t-1)\leq d^q(t)\leq a^q(t)
\Big\} \nonumber
\label{ex-ante}
\min_{B(t),M(t)} \sum_{t\in \Omega}{\mathbb E}\{{\mathcal C}^{F}(L(t),B(t),M(t))\}~~\mbox{s.t.}~ L(t)\in { \mathcal L}^{DR}(t),
\label{myopic}
\min_{L(t)} ~{\mathcal C}^R(L(t),B(t),M(t))~~\mbox{s.t.}~ L(t)\in { \mathcal L}^{DR}(t),
{\mathcal L}^{DR}(t) = {\mathcal L}(t).
{\mathcal L}^{DR}(t) = \big\{ L(t) |& L(t) = f(t;\mathbf{p}(t)), \mathbf{p}(t) \in \mathcal{Z}(t) \big\}
\label{priceresp}
 f(t;\mathbf{p}(t)) = \mbox{argmin}_{L(t) \in \mathcal{L}(t)} \sum_{t = 1}^{\tau} \pi(t) L(t).

{\kappa}_{x,x'}^q(t) = \frac{d_{x,x'}^q(t)}{n_x^q(t)},~~x'\in \mathcal S_x

{\kappa}_{x}^q(t) = \frac{n_{x,1}^q(t)}{n_x^q(t)}
\label{alpha2}
\tau^q(t)=\min\lbrace t' \leq t: a^q(t') \geq d^q(t)\rbrace.

{\kappa}^q(t) = \frac{ a^q(t') - d^q(t)}{\partial a^q(t')}
\label{rate}
p_i(t)=\mathbb{E}\{\partial a_i(t)\}.
 \label{ratemac}\rho_{\mathcal N}(t)=\delta T^{-1}\sum_{i\in {\mathcal N}}p_i(t)\prod_{j\in {\mathcal N}/i}(1-\alpha p_j(t)).
\boldsymbol{L}_i=\boldsymbol{L}^I_i+\boldsymbol{L}^F_i 

\log p_{\boldsymbol{L}^I_i}(\boldsymbol{L}_i-\boldsymbol{L}_i^{DR} )\geq \eta
\|\boldsymbol{L}_i-\boldsymbol{L}_i^{DR}-\boldsymbol{\mu}_{\boldsymbol{L}^I_i}\|^2_{\boldsymbol{W}_{\boldsymbol{L}^I_i}^{-1}}\leq \eta'.
\min_{B(h)} \sum_{h=1}^H & {\mathbb E} ~\{ {\mathcal C}^{F}(L(t);B(h))\} = \label{dacost}\\ 
\min_{B(h)} \sum_{h=1}^H &\bigg\{ \pi^{F}(h) B(h) +  {\mathbb E}\{ {\mathcal C}^{R}(L(t);B(h)) \}  \bigg\}\nonumber\\
\mbox{s.t.}~~~~~& L(t)\in { \mathcal L}(t),\nonumber
\label{rtcost}
&{\mathcal C}^{R}(L(t);B(h)) =\\ &\sum_{h=1}^{H} \sum_{\ell = 1}^T \big\{ \pi^{R}_{up}((h-1)T+\ell) (L((h-1)T+\ell) - B(h))^+ \nonumber\\ &~~~~~~~~~~+\pi^{R}_{dn}((h-1)T+\ell) (L((h-1)T+\ell) - B(h))^- \big\}. \nonumber 
{\mathcal L}^v(h) = \Big\{L(h)|&  L(h) = \sum_{q=1}^{32} \sum_{x=0}^{5} \sum_{x'=0}^{5}(x'-x)\partial d^q_{x,x'}(h),\nonumber\\ &\partial d_{x,x'}^q(h) \in \mathbb{Z}^+,\!\! \sum_{x=0}^{5}\partial d_{x,x'}^q(h)\leq n^q_x(h),\nonumber \\&  n_x^q(q) = 0, \forall x < 5\Big\},\label{tank}

{\mathbb E}[L^{\rm base}(h)] = \sum_{q=1}^Q n^q(h) G^q\frac{ \tau_{\rm on}^{q}(h)}{\tau_{\rm on}^{q}(h) + \tau_{\rm off}^{q}(h)},\\
n^q(h)={\mathbb E}\left[\sum_{x\in {\mathcal S}} \sum_{\ell=1}^T n^q_x((h-1)T + \ell)\right],

 \tau_{\rm on}^{q}(h)&=\frac{1}{k^q} \ln\left(
\frac{x^{*q}-\frac{B^q} 2 -\frac{G^q}{k^q}-x_{\rm amb}^q(h)}
{x^{*q}+\frac{B^q} 2-\frac{G^q}{k^q}-x_{\rm amb}^q(h)}
\right),\\
 \tau_{\rm off}^{q}(h)&=\frac{1}{k^q} \ln\left(
\frac{x^{*q}+\frac{B^q} 2 -x_{\rm amb}^q(h)}
{x^{*q}-\frac{B^q} 2 -x_{\rm amb}^q(h)}
\right).
 
{\mathbb E}[L^{\rm max}(h)] = \sum_{q=1}^Q n^q(h) G^q\frac{ \tau_{\rm on}^{q,\max}(h)}{\tau_{\rm on}^{q,\max}(h) + \tau_{\rm off}^{q,\min}(h)},
 \tau_{\rm on}^{q,\max}(h)&=\frac{1}{k^q} \ln\left(
\frac{x^{*q}+\frac{B^q} 2 - \Theta-\frac{G^q}{k^q}-x_{\rm amb}^q(h)}
{x^{*q}+\frac{B^q} 2-\frac{G^q}{k^q}-x_{\rm amb}^q(h)}
\right),\\
 \tau_{\rm off}^{q,\min}(h)&=\frac{1}{k^q} \ln\left(
\frac{x^{*q}+\frac{B^q} 2 -x_{\rm amb}^q(h)}
{x^{*q}+\frac{B^q} 2 - \Theta-x_{\rm amb}^q(h)}
\right).
 
{\mathbb E}[L^{\rm min}(h)] = \sum_{q=1}^Q n^q(h) G^q\frac{ \tau_{\rm on}^{q,\min}(h)}{\tau_{\rm on}^{q,\min}(h) + \tau_{\rm off}^{q,\max}(h)},

M \!\!=\!\! \min_h \min{\mathbb E}\{L^{\rm base}(h) \!-\! L^{\rm min}(h),  L^{\rm max}(h) \!-\!  L^{\rm base}(h)\}.

M' =  \sum_{q=1}^Q  \min_{h}n^q(h) M^q(h),

\sum_{x=0}^{E}\sum_{x'=x}^{E} &\partial n_{x'}(t) = \\&~\sum_{x=0}^{E} \sum_{x'=x}^{E}\sum_{i\in {\cal P}} \delta(x_i(t+1)-x')a_i(t+1)\\
		      &-\sum_{x=0}^{E} \sum_{x'=x}^{E} \sum_{i\in {\cal P}}\delta(x_i(t)-x')a_i(t)\\
		      &=\sum_{i\in {\cal P}}\sum_{x=0}^{E}u(x_i(t)+\partial x_i(t)-x)(a_i(t)+\partial a_i(t))\\
		      &-\sum_{i\in {\cal P}}\sum_{x=0}^{E}u(x_i(t)-x)a_i(t)\\
		      &=\sum_{i\in {\cal P}}\sum_{x=0}^{E} [u(x_i(t)+\partial x_i(t)-x)-u(x_i(t)-x)]a_i(t)\\
		      &+\sum_{i\in {\cal P}}\sum_{x=0}^{E}u(x_i(t+1)  -x)\partial a_i(t)\\
		      &= \sum_{i\in {\cal P}}\partial x_i(t) a_i(t)+ \sum_{i\in {\cal P}} (x_i(t+1)+1) \partial a_i(t) \\
		      &=\sum_{i\in {\cal P}}L_i(t)+ \sum_{i\in {\cal P}} (S_i+1) \partial a_i(t)  \\
&=L(t)+ \sum_{x=0}^{E} (x+1) \partial a_x(t).

The second to last equality holds following \eqref{pop} and the fact that  is only non zero when , i.e., .
\end{proof}

\bibliographystyle{IEEEtran}
\small
\bibliography{New2,new4,new5,newrefs}

\end{document}
