\documentclass[letterpaper,singlecolumn,9pt]{sig-alternate-2013}

\usepackage[T1]{fontenc}
\usepackage[utf8]{inputenc}
\usepackage{t1enc}

\usepackage{amsmath}
\usepackage{amsfonts}
\usepackage{amssymb}



\usepackage{multirow,bigdelim}
\usepackage{rotating}
\usepackage{caption}
\usepackage[hang]{subfigure}
\usepackage{algorithm}
\usepackage[noend]{algpseudocode}
\usepackage[]{units}

\usepackage{tikz}
\usepackage{gnuplot-lua-tikz}
\usepackage{cite}
\usepackage{url}
\usepackage{xspace}
\usepackage{multicol}
\usepackage{ifpdf}



\newtheorem{proposition}{Proposition}
\newtheorem{theorem}{Theorem}
\newtheorem{definition}{Definition}
\newtheorem{lemma}{Lemma}
\newtheorem{corollary}{Corollary}

\usepackage{bigfoot}



\newcommand{\abs}[1]{\lvert #1 \rvert}
\DeclareMathOperator*{\argmin}{argmin}
\DeclareMathOperator{\polylog}{polylog}
\DeclareMathOperator{\mbw}{mbw}
\DeclareMathOperator{\last}{last}
\DeclareMathOperator{\lp}{lp}
\DeclareMathOperator{\Find}{find}
\DeclareMathOperator{\Delete}{delete}
\DeclareMathOperator{\newid}{new\_id}
\DeclareMathOperator{\NULL}{NULL}
\DeclareMathOperator{\level}{level}
\DeclareMathOperator{\xbwl}{xbwb}
\DeclareMathOperator{\pDAG}{pDAG}

\DeclareMathOperator{\access}{access}
\DeclareMathOperator{\rank}{rank}
\DeclareMathOperator{\select}{select}
\DeclareMathOperator{\getbits}{bits}
\DeclareMathOperator{\leafpush}{leaf\_push}

\newcommand{\XBWL}{\emph{XBW-b}\xspace}
\newcommand{\stind}{\ensuremath{\mathcal{S}}}
\newcommand{\M}{\mathcal M}
\newcommand{\refc}{\ensuremath{\text{ref\_count}}}
\newcommand{\Left}{\ensuremath{\text{left}}}
\newcommand{\Right}{\ensuremath{\text{right}}}
\newcommand{\parent}{\ensuremath{\text{parent}}}
\newcommand{\id}{\ensuremath{\text{id}}}
\newcommand{\Root}{\ensuremath{\text{root}}}
\newcommand{\Replace}{\ensuremath{\text{replace}}}
\newcommand{\Copy}{\ensuremath{\text{copy}}}
\newcommand{\New}{\ensuremath{\text{new\_node}}}

\newcommand{\lambertW}{\ensuremath{\mathcal{W}}}

\newcommand{\lookup}{\ensuremath{\texttt{lookup}}}
\newcommand{\lookupnode}{\ensuremath{\texttt{lookup\_node}}}
\newcommand{\copytree}{\ensuremath{\texttt{copy\_tree}}}
\newcommand{\triefold}{\ensuremath{\texttt{trie\_fold}}}
\newcommand{\update}{\ensuremath{\texttt{update}}}
\newcommand{\compress}{\ensuremath{\texttt{compress}}}
\newcommand{\decompress}{\ensuremath{\texttt{decompress}}}
\newcommand{\Put}{\ensuremath{\texttt{put}}}
\newcommand{\Get}{\ensuremath{\texttt{get}}}

\DeclareNewFootnote[para]{default}
\DeclareNewFootnote[para]{E}[alph]
\MakeSortedPerPage{footnoteE}
\interfootnotelinepenalty=10000

\allowdisplaybreaks[4]

\newcommand*{\plogo}{\fbox{}} 

\newcommand*{\titlePage}{\begingroup 

\onecolumn
\centering 

\begin{center}
  \includegraphics[width=200pt]{BME1782nagy.eps}
\end{center}

\vspace*{6\baselineskip} 

{\Huge Compressing IP Forwarding
     Tables:\0.2\baselineskip] 

\vspace*{\baselineskip} 

{\Huge A revised technical report}\\baselineskip]

\vspace*{10\baselineskip} 

Authors \\label{eq:Shannon-entropy}
    H_0 = \sum_{s\in\Sigma} p_s \log_2\nicefrac1{p_s} \enspace  .
  
    \label{eq:leaf-push-barrier-delta}
    \lambda = \Big \lfloor \frac1{\ln 2} \lambertW\left( n \ln \delta
    \right) \Big \rfloor \enspace ,
  
    \label{eq:leaf-push-barrier-H0}
    \lambda = \Big \lfloor  \frac1{\ln 2} \lambertW(n H_0 \ln 2)  \Big
    \rfloor \enspace .
  \label{eq:kappa}
    \kappa 2^{\kappa} = 2^{W} \log_2(\delta) = n \log_2(\delta) \enspace .  
  \sum_{j=0}^{\lambda} \abs{V^j_D} = \sum_{j=0}^{\lambda} 2^j=
  2^{\lambda+1}-1\leq2\cdot2^{\kappa}
    \left(2 +2\left(1+ \frac{2}{\sqrt{2^{\kappa}}} \right)\right) \lceil
    \kappa
    \rceil 2^{\kappa} + \left(2\cdot2^\kappa+\delta\right)\log_2\delta\\
    =4 n \log_2(\delta) + o(n)
  \label{eq:vjd-ub}
    E(|V^j_D|) \leq \min\left\{2^{j}, \ \frac{H_0}{j} 2^{W} + 3,\ \delta^{2^{W-j}} \right\} \enspace .
  \label{size-head-node}
    \sum_{j=0}^{\lfloor\xi\rfloor}  E(|V^j_D|) \leq \sum_{j=0}^{\lfloor\xi\rfloor}  2^{j} = 2^{\lfloor\xi\rfloor+1}-1\\
    <2 \cdot 2^{\xi} = 2\left( \frac{H_0}{\xi} 2^{W} + 3\right) =2 M
  \label{size-tail-node}
    \sum_{j=\lceil\zeta\rceil}^{W}& E(|V^j_D|) \leq
    \sum_{j=\lceil\zeta\rceil}^{W} \delta^{2^{W-j}} =
    \sum_{j=1}^{W-\lceil\zeta\rceil} \delta^{2^{j}} \notag\\
    &=\delta^{2^{W-\lceil\zeta\rceil}} + \sum_{j=1}^{W-\lceil\zeta\rceil-1}
    \delta^{2^{j}}
    < \delta^{2^{W-\zeta}} + \sum_{i=1}^{2^{W-\lceil\zeta\rceil-1}}  \delta^{i}\notag\\
    &= \delta^{2^{W-\zeta}} + \delta^{2^{W-\lceil\zeta\rceil-1}+1}-2
    < \delta^{2^{W-\zeta}} + \delta \sqrt{\delta^{2^{W-\zeta}}}\notag\\
    &= \delta^{2^{W-\zeta}} \left(1 +
      \frac{\delta}{\sqrt{\delta^{2^{W-\zeta}}}}
    \right)=\left(\frac{H_0}{\zeta} 2^{W} + 3 \right) \left(1 + \epsilon_1
    \right)\notag\\
    &< \left(\frac{H_0}{\xi} 2^{W} + 3 \right) \left(1 + \epsilon_1 \right) =
    M(1+\epsilon_1) \enspace ,
  
    \epsilon_1 = \frac{\delta}{\sqrt{\delta^{2^{W-\zeta}}}} \le
    \frac{\delta}{\sqrt{\delta^{\frac{W-\log_2\nicefrac{W}{H_0}}{\log_2\delta}}}}=\frac{\delta\sqrt{\nicefrac{W}{H_0}}}{2^{W/2}}
    \enspace , 
  
    \sum_{j=\lfloor\xi\rfloor+1}^{\lceil\zeta\rceil-1} E(|V^j_D|) \leq
    \sum_{j=\lfloor\xi\rfloor+1}^{\lceil\zeta\rceil-1} \left(\frac{H_0}{j}
      2^{W} + 3 \right) <\\
    < \sum_{j=\lfloor\xi\rfloor+1}^{\lceil\zeta\rceil-1}
    \left(\frac{H_0}{\xi} 2^{W} + 3 \right)
    =(\lceil\zeta\rceil-1-\lfloor\xi\rfloor) M\\
    \le (\zeta-(\xi-1)) M = (1+\zeta-\xi) M \enspace .
  
      \xi &\geq & W-\log_2\nicefrac{W}{H_0} \enspace ,\label{eq:bound_on_xi}\\
      \zeta &\leq& W - \log_2 \left(W-\log_2 \nicefrac{W}{H_0} \right)+\log_2\log_2(\delta) \enspace ,\label{eq:bound_on_zeta}\\
      \kappa&\le&  W-\log_2\left(W-\log_2W\right)+\log_2\log_2\delta \enspace .\label{eq:bound_on_kappa}
    \label{size-body-node}
    &\phantom{=}\sum_{j=\lfloor\xi\rfloor+1}^{\lceil\zeta\rceil-1}E(|V^j_D|) \leq(1+\zeta-\xi) M\notag\\
    &\le\left(1+ \log_2 \left( \frac{W}{H_0} \right) - \log_2
      \left({\frac{W-\log_2 \left( \frac{W}{H_0}
            \right)}{\log_2(\delta)}}\right) \right) M\notag\\
    &=\left(1 + \log\log_2(\delta)-\log_2H_0 + \epsilon_2\right) M,
  
    \epsilon_2=\log_2  \frac{W}{W -\log_2 \left( \frac{W}{H_0} \right)}
    \xrightarrow[W\to\infty]{} 0 \enspace .
  
    \left(2 + 2(1+\epsilon) +2\left(1-\log_2
        H_0+\log\log_2(\delta)+\epsilon_2\right)\right)M \\= \left(6+2\log_2
      \frac{\log_2\delta}{H_0}+2\left(\epsilon_1+\epsilon_2\right)\right)M
    \enspace .
  
    \left(6+2\log_2
      \frac{\log_2\delta}{H_0}+2\left(\epsilon_1+\epsilon_2\right)\right)M\lceil\kappa\rceil+\left(2M+\delta\right)\log_2\delta
    \enspace . 
  
    &\phantom{=}M\lceil\kappa\rceil =
    \lceil\kappa\rceil\left(\frac{H_0}{\xi}2^W+3\right)\le
    \frac{\kappa+1}{\xi}H_0 n + 3\lceil\kappa\rceil\\
    &\le\left( \frac{W-\log_2\frac{W-\log_2 W}{\log_2\delta}+1}{W-\log_2\nicefrac{W}{H_0}}\right)H_0n + 3\lceil\kappa\rceil=\\
    &= \left(1+\frac{\log_2\nicefrac{W}{H_0}-\log_2\frac{W-\log_2
          W}{\log_2\delta}+1}{W-\log_2\nicefrac{W}{H_0}}\right)H_0n +
    3\lceil\kappa\rceil\\
    &=H_0n+o(n) \enspace.
  
    \frac{n\log_2\delta}{\kappa}=2^\kappa\le\frac{H_0}{\kappa}n+3\enspace.
  \label{eachp}
      p_o< \frac 1e \Rightarrow 1-(1-p_o)^m \leq \frac{m}{\log_2(m)} p_o \log_2 \frac{1}{p_o} \enspace .
    
        1-(1-p_o)^m \leq 1 = \frac{1/p_o}{\log_2(1/p_o)} p_o \log_2
        \frac{1}{p_o} \leq \frac{m}{\log_2(m)} p_o \log_2 \frac{1}{p_o}
        \enspace .
      
        1-(1-p_o)^{\frac1{p_o^x}} \leq
        \frac{\frac1{p_o^x}}{\log_2\left({\frac1{p_o^x}}\right)} p_o \log_2
        \left(\frac{1}{p_o}\right) =
         \\
         = \frac{\frac1{p_o^x}}{x
         \log_2\left({\frac1{p_o}}\right)} p_o \log_2
         \left(\frac{1}{p_o}\right) = \frac{\frac1{p_o^x}}{x} p_o =
        \frac1{xp_o^{x-1}} \enspace .
       
       (1-p_o)^{\frac1{p_o^x }}\geq 1 - \frac1{xp_o^{x-1}} \enspace.
      \label{reducedeq} (1-p_o)^{\frac1{p_o}}\geq \left({1 -
           \frac1{xp_o^{x-1}}}\right)^{p_o^{x-1}} .
     
    (1-p_o)^{\frac1{p_o}}\geq \left({1 - \frac1{p_o^{x-1}}}\right)^{p_o^{x-1}}.
      \label{k-bounds}
       2^{l} = 2^{W-\log_2  \nicefrac{W}{H_0} } \leq 2^{W-\log_2 
         \nicefrac{W}{H_0}} = 2^W\frac{H_0}{W}  < \frac{H_0}{l} 2^{W} + 3
       \enspace .
      \label{l-bounds} \delta^{2^{W-l}} = \delta^{
         \frac{W-\log_2 \left( \frac{W}{H_0} \right)}{\log_2(\delta)} }=
       \delta^{\frac{\log_2 \left( \frac{H_0}{W} 2^W\right)}{\log_2(\delta)}
       }\\
       =\frac{H_0}{W} 2^W < \frac{H_0}{l} 2^{W} + 3 \enspace .
  
    \delta^{2^{W-l}}=\delta^\frac{W-\log_2W}{\log_2\delta}=2^{W-\log_2W}\le2^{l}
    \enspace . 
  

  This completes the proof.
\end{proof}

\end{document}
